common/EventsAux.v
@@ -1,0 +1,341 @@
+
+Require Import String.
+Require Import Coqlib.
+Require Intv.
+Require Import AST.
+Require Import Integers.
+Require Import Floats.
+Require Import Values.
+Require Import Memory.
+Require Import Globalenvs.
+
+
+Lemma Forall2_impl:
+  forall {A B} (r1 r2:A-> B -> Prop) l1 l2, (forall a b, r1 a b -> r2 a b) ->
+          Forall2 r1 l1 l2 -> Forall2 r2 l1 l2.
+Proof.
+  intros until l1; induction l1.
+  - intros * ? H; inv H; constructor.
+  - intros * ? H; inv H; constructor; eauto.
+Qed.
+
+(* New strong injection. This relation is injective! *)
+Inductive inject_strong (mi : meminj) : val -> val -> Prop :=
+    inject_int : forall i : int, inject_strong mi (Vint i) (Vint i)
+  | inject_long : forall i : int64, inject_strong mi (Vlong i) (Vlong i)
+  | inject_float : forall f : float, inject_strong mi (Vfloat f) (Vfloat f)
+  | inject_single : forall f : float32, inject_strong mi (Vsingle f) (Vsingle f)
+  | inject_ptr : forall (b1 : block) (ofs1 : ptrofs) (b2 : block) (ofs2 : ptrofs) (delta : Z),
+                 mi b1 = Some (b2, delta) ->
+                 ofs2 = Ptrofs.add ofs1 (Ptrofs.repr delta) ->
+                 inject_strong mi (Vptr b1 ofs1) (Vptr b2 ofs2)
+  | val_inject_undef : inject_strong mi Vundef Vundef.
+Inductive memval_inject_strong (f : meminj) : memval -> memval -> Prop :=
+    memval_inject_byte_str : forall n : byte, memval_inject_strong f (Byte n) (Byte n)
+  | memval_inject_frag_str : forall (v1 v2 : val) (q : quantity) (n : nat),
+                         inject_strong f v1 v2 ->
+                         memval_inject_strong f (Fragment v1 q n) (Fragment v2 q n)
+  | memval_inject_undef_str : memval_inject_strong f Undef Undef.
+                                              
+Definition list_memval_inject mu:= Forall2 (memval_inject mu).
+Definition list_memval_inject_strong mu:= Forall2 (memval_inject_strong mu).
+Lemma memval_inject_strong_weak:
+         forall f v1 v2, memval_inject_strong f v1 v2 ->  memval_inject f v1 v2.
+Proof. intros * HH; inv HH; econstructor; auto. inv H; econstructor; eauto. Qed.
+Lemma list_memval_inject_strong_weak:
+  forall f vals1 vals2, list_memval_inject_strong f vals1 vals2 ->
+                   list_memval_inject f vals1 vals2.
+Proof. intros *; eapply Forall2_impl; apply memval_inject_strong_weak. Qed.
+
+(*Injection for block ranges*)
+Inductive inject_hi_low (mu:meminj): (block * Z * Z) -> (block * Z * Z) -> Prop:=
+| HiLow: forall b1 b2 hi low delt,
+    mu b1 = Some(b2, delt) ->
+    inject_hi_low mu (b1, hi, low) (b2, hi+delt, low+delt).
+Definition list_inject_hi_low mu := Forall2 (inject_hi_low mu).
+  
+(*
+  Delta Permission Maps:
+  A change in memory permissions.
+  - They have the same shape as the memories
+  - they return [None], if the permission doesn't change at that location
+  - return [Some perm], if the new permission is [perm].
+*)
+Notation delta_perm_map := (Maps.PTree.t (Z -> option (option permission))).
+Definition inject_Z_map {A} (delt: Z) (f1 f2: (Z -> option A)): Prop:=
+  forall ofs p, f1 ofs = Some p -> f1 ofs = f2 (ofs+ delt).
+    
+Record inject_delta_map (mu: meminj)(dpm1 dpm2: delta_perm_map): Prop:=
+  { DPM_image: (*All permissions changed are mapped*)
+      forall b1 f1, (Maps.PTree.get b1 dpm1) = Some f1 ->
+      exists b2 delt f2, mu b1 = Some (b2, delt) /\
+                     Maps.PTree.get b2 dpm2 = Some f2 /\
+            inject_Z_map delt f1 f2
+    ;DPM_preimage:
+       forall b2 ofs2 f2 p,
+         Maps.PTree.get b2 dpm2 = Some f2 ->
+         f2 ofs2 = p ->
+         exists b1 f1 ofs1 delt,
+           mu b1 = Some(b2, delt) /\
+           Maps.PTree.get b1 dpm1 = Some f1 /\
+           f1 ofs1 = p /\
+           ofs2 = ofs1 + delt
+  }.
+
+
+
+
+
+
+
+
+(** *Relations that are monotonic w.r.t. injections*)
+Definition inj_monotone{A} (R:meminj -> A -> A-> Prop):Prop:=
+  forall (a b:A) f f',  R f a b -> inject_incr f f' -> R f' a b.
+Lemma Forall2_incr:
+  forall {A} (R: meminj -> A -> A -> Prop),
+    inj_monotone R ->
+    inj_monotone (fun j => Forall2 (R j)).
+Proof.
+  intros A R HR; unfold inj_monotone.
+  induction a; intros ? ? ? HH; inv HH; intros; constructor; eauto.
+Qed.
+Create HintDb inj_mono. Hint Resolve Forall2_incr: inj_mono.
+Ltac inj_mono_tac:=
+  match goal with
+    [|- inj_monotone ?R ] =>
+    (* If it's a list try the list lemma *)
+    try (eapply Forall2_incr; eauto with  inj_mono);
+    intros ???? ?HR ?Hincr; inv HR;
+    try solve[econstructor; eauto with inj_mono]
+  | _ => fail "Expected goal: inj_monotone ?R" 
+  end.
+
+
+
+
+
+
+
+
+(** * Relations that compose with injections *)
+Definition composes_inj {A} (R: meminj -> A -> A ->Prop):=
+  forall j12 j23 x1 x2 x3, R j12 x1 x2 -> R j23 x2 x3 -> R (compose_meminj j12 j23) x1 x3.
+Create HintDb compose_inj.
+Lemma Forall2_compose:
+  forall {A} (R: meminj -> A -> A -> Prop),
+    composes_inj R -> composes_inj (fun j => Forall2 (R j)).
+Proof.
+  intros ** ?? ls. induction ls; intros * H0 H1;
+  inv H0; inv H1; constructor; eauto.
+Qed.
+Hint Resolve Forall2_compose: compose_inj.
+Ltac composition_arithmetic:=
+  (* Solves the Ptrofs.add... goal that results from 
+       injecting a pointer twice: the offsets are added 
+       in two different ways *)
+  rewrite Ptrofs.add_assoc; decEq;
+  unfold Ptrofs.add; apply Ptrofs.eqm_samerepr; auto with ints.
+Ltac composed_injections_injection_case j12 j23:=
+  match goal with
+  |[ H12: j12 _ = Some _, H23: j23 _ = Some _ |-
+     context[compose_meminj j12 j23] ] =>
+   econstructor;
+   try (unfold compose_meminj; rewrite H12; rewrite H23); eauto;
+   try composition_arithmetic; eauto with compose_inj
+  end.
+Ltac composed_injections:=
+  match goal with
+  |[|- composes_inj ?R] =>
+   let H1:= fresh "H1" in let H2:= fresh "H2" in 
+                          intros j12 j23  ??? H1 H2;
+                          inv H1; auto; inv H2; auto;
+                          try solve[econstructor; eauto with compose_inj];
+                          try composed_injections_injection_case j12 j23
+  | _ => fail "Not the shape expected"
+  end.
+Ltac rewrite_compose_meminj:=
+  match goal with
+  |[ H12: ?j12 _ = Some _, H23: ?j23 _ = Some _ |-
+     context[compose_meminj ?j12 ?j23]
+   ] => unfold compose_meminj; rewrite H12, H23
+  end.
+
+
+  Lemma inject_delta_map_compose: composes_inj inject_delta_map.
+Proof. intros ? **.
+       inv H; inv H0.
+       constructor.
+       - intros; exploit  DPM_image0; eauto.
+         intros (?&?&?&?&?&?).
+         exploit  DPM_image1; eauto.
+         intros (?&?&?&?&?&?).
+         repeat (econstructor; eauto).
+         unfold compose_meminj;
+           rewrite H0, H3; reflexivity.
+         intros ** ofs. 
+         intros ??HH.
+         erewrite H2; eauto.
+         erewrite H5; eauto. f_equal. omega.
+         rewrite <- HH. exploit H2; eauto.
+       - intros; exploit  DPM_preimage1; eauto.
+         intros (?&?&?&?&?&?&?&?).
+         exploit  DPM_preimage0; eauto.
+         intros (?&?&?&?&?&?&?&?).
+         repeat (econstructor; eauto).
+         unfold compose_meminj; rewrite H5, H1; reflexivity.
+         subst; eauto; omega.
+Qed.
+Hint Resolve inject_delta_map_compose: compose_inj.
+
+Lemma inject_hi_low_compose: composes_inj inject_hi_low.
+Proof. composed_injections; do 2 rewrite Zplus_assoc_reverse.
+       econstructor; rewrite_compose_meminj; reflexivity. Qed.
+Hint Resolve inject_hi_low_compose:compose_inj. 
+Lemma list_inject_hi_low_compose: composes_inj list_inject_hi_low.
+Proof. eauto with compose_inj. Qed.
+Hint Resolve list_inject_hi_low_compose:compose_inj. 
+
+
+
+(** *Strong interpolation:
+    An injection relation, induced by a composed meminj,
+    can be split into a strong one and a regular one.
+*)
+  Definition strong_interpolation {A} (R: meminj -> A -> A -> Prop)
+             (R_strong: meminj -> A -> A -> Prop):=
+    forall v1 v3 j12 j23, R (compose_meminj j12 j23) v1 v3 ->
+      exists v2,  R_strong j12 v1 v2 /\ R j23 v2 v3.
+  Create HintDb str_interp.
+  Ltac case_compose_meminj:=
+    match goal with
+    | [ H: compose_meminj ?f1 ?f2 ?b = Some _  |- _ ] =>
+      unfold compose_meminj in H; repeat match_case in H;
+      subst;
+      try match goal with
+          | [ H: Some _ = Some _ |- _ ] => inv H
+          end
+    end.
+  (* apply a strong interpolation lemma in a hypothesis*)
+  Lemma list_str_interpol:
+    forall {A} (R R_str: meminj -> A -> A -> Prop) ,
+      strong_interpolation R R_str ->
+      strong_interpolation (fun f => Forall2 (R f))
+                           (fun f => Forall2 (R_str f)).
+Proof.
+  intros.
+  unfold strong_interpolation.
+  induction v1; intros.
+  - inv H0; do 3 econstructor. 
+  - inv H0.
+    exploit IHv1; eauto. intros (?&?&?).
+    exploit H; eauto. intros (?&?&?).
+    do 3 econstructor; eauto.
+Qed.
+Lemma str_interpol_cut:
+  forall A R R_str,
+    @strong_interpolation A R R_str -> 
+    @strong_interpolation A R R_str.
+Proof. eauto. Qed.
+Ltac use_interpolations_in_hyps:=
+  match goal with
+  | [ H: ?R (compose_meminj ?j12 ?j23) _ _ |- _ ] =>
+    eapply (@str_interpol_cut _ R) in H;
+    [ destruct H as (?&?&?) | solve[eauto with str_interp]]
+  end.
+Ltac str_interp:=
+  match goal with
+    [|- strong_interpolation ?R ?R_Str] =>
+    (* try if it's a list*)
+    try (eapply list_str_interpol;
+         eauto with str_interp);
+    intros ???? ?HR; inv HR;
+    try case_compose_meminj;
+    (* exploit one interpolation from the hypothesis *)
+    repeat use_interpolations_in_hyps;
+    (*try easy cases *)
+    try solve[ do 3 econstructor];
+    try solve[repeat (econstructor; eauto with str_interp)]
+  end.
+
+Lemma inject_delta_interpolation: strong_interpolation inject_delta_map inject_delta_map.
+Proof.
+  str_interp.
+  remember (Maps.PTree.elements v1) as ls1.
+  set (mapped_delta:= fun {A} (j:meminj) (ls: list (positive * (Z -> A))) =>
+                        @fold_left (Maps.PTree.t _) (positive * _)
+                          (fun dmap b1_f1 =>
+                             let (b1, f):= b1_f1 in
+                             match j b1  with
+                             | Some (b2, delt) =>
+                               Maps.PTree.set
+                                 b1 (fun ofs => f (ofs - delt)) dmap
+                             | _ => dmap
+                                     end)
+                          ls (Maps.PTree.empty (Z -> A))).
+       exists (mapped_delta _ j12 ls1); split.
+       - econstructor; intros.
+         + exploit DPM_image0; try eassumption;
+             intros (?&?&?&?&?&?).
+           case_compose_meminj.
+           repeat (econstructor; eauto).
+           
+           
+
+Admitted.
+Hint Resolve inject_delta_interpolation: str_interp.
+
+
+
+(** *Determinism in relations *)
+Definition deterministic {A B} (R: A -> B -> Prop):=
+    forall a b b', R a b -> R a b' -> b = b'.
+  Lemma determ_cut:
+    forall A B R, @deterministic A B R -> deterministic R. Proof. eauto. Qed.
+  Lemma  Forall2_determ:
+    forall {A B} (R: A -> B -> Prop),
+      deterministic R ->
+      deterministic (Forall2 R).
+  Proof.
+    unfold deterministic;
+      intros. revert b' H1.
+    induction H0; intros.
+    - inv H1; auto.
+    - inv H2; f_equal.
+      + eapply H; eassumption.
+      + eapply IHForall2; assumption.
+  Qed.
+  Create HintDb determ. Hint Resolve Forall2_determ: determ.
+  
+    Ltac different_results:=
+      match goal with
+        [H: ?a = _, H0: ?a = _ |- _]=>
+        rewrite H in H0; inv H0
+      end.
+    Ltac determ_hyp:=
+      match goal with
+        [H: ?R ?a ?b, H0: ?R ?a ?b' |- _] =>
+        replace b with b' in * by (eapply determ_cut; eauto with determ);
+        auto; clear H0
+      end.
+    Ltac solve_determ:=
+      match goal with
+        [|- forall j,  deterministic ?R ] =>
+        let H:= fresh in let H0:=fresh in
+        eauto with determ;
+        intros ?? * H H0; inv H; inv H0;
+        repeat different_results;
+        repeat determ_hyp;
+        eauto
+      end.
+    Lemma inject_delta_map_determ:
+    forall (f12 : meminj), deterministic (inject_delta_map f12).  
+  Proof. solve_determ.
+  Admitted.
+  Hint Resolve inject_delta_map_determ: determ.
+
+
+
+  (** *Some trivial hints added to the database. *)
+  Hint Immediate inject_incr_refl.
+  
